

$$1. m(a+bx) = a + b \cdot m(x)$$

$$\frac{1}{N} \sum_{i=1}^N (a + bx_i) = a + b m(x)$$

$$\frac{1}{N} \sum_{i=1}^N a + \frac{1}{N} \sum_{i=1}^N bx_i$$

$$\frac{1}{N} aN + \frac{b}{N} \sum_{i=1}^N x_i = a + b m(x)$$

$$a + b m(x) = a + b m(x)$$

$$2. \text{cov}(X, a+bY)$$

$$= \frac{1}{N} \sum_{i=1}^N (x_i - m(x)) (a + bY_i - m(a+bY))$$

$$= \frac{1}{N} \sum_{i=1}^N (x_i - m(x)) (a + bY_i - a - b m(Y))$$

$$= \frac{1}{N} \sum_{i=1}^N (x_i - m(x)) b (Y_i - m(Y))$$

$$= \frac{b}{N} \sum_{i=1}^N (x_i - m(x)) (Y_i - m(Y))$$

$$= b \text{cov}(X, Y)$$

$$3. \text{cov}(a+bx, a+bx)$$

$$= \frac{1}{N} \sum_{i=1}^N (a+bx_i - m(a+bx)) (a+bx_i - m(a+bx))$$

$$= \frac{1}{N} \sum_{i=1}^N (a+bx_i - a - bm(x)) (a+bx_i - a - bm(x))$$

$$= \frac{1}{N} \sum_{i=1}^N b^2 (x_i - m(x)) (x_i - m(x))$$

$$= \frac{b^2}{N} \sum_{i=1}^N (x_i - m(x)) (x_i - m(x)) = \frac{b^2}{N} \sum_{i=1}^N (x_i - m(x))^2 = b^2 s^2$$

$$= b^2 \text{cov}(x, x)$$

$$\text{if } b=1:$$

$$\text{cov}(x, x) = s^2$$

$$4. x = (1, 2, 3)$$

$$\text{Median}(x) = [1]$$

$$3-1 = 2$$

$$g(x) = 2+5x = (7, 12, 17)$$

$$\text{Median}(g) = [1] = 2+5\text{Median}(x)$$

$$17-7 = 10$$

$$h(x) = \text{arcsinh}(x) = (.88, 1.44, 1.82)$$

$$\text{Median}(h) = [1] = \text{arcsinh}(\text{Median}(x))$$

$$1.82 - .88 = .94$$

Any nondecreasing transformation doesn't affect the order so median will be the same. Same applies to any quantile but not IQR or range since distance will be affected.

$$5. m(g(x)) = \frac{7+12+17}{3} = 12$$

$$m(h(x)) = \frac{.88+1.44+1.82}{3} = 1.38$$

$$g(m(x)) = 2+5(2) = 12$$

$$h(m(x)) = \text{arcsinh}(2) = 1.44$$

Not true that $m(g(x)) = g(m(x))$, but can be true sometimes.